concurrency/DryMachineSource.v
@@ -349,9 +349,9 @@ Module THE_DRY_MACHINE_SOURCE.
 
       (*Compute the bounds*)
       assert (Hbound':=Hbound).
-      eapply bounded_maps.finite_sub_maps with (A:= (option permission))
+      eapply bounded_maps.finite_sub_maps
         in Hbound as bounded_delta_map.
-      eapply bounded_maps.finite_sub_maps with (A:=permission)
+      eapply bounded_maps.finite_sub_maps
         in Hbound' as bounded_access_map.
 
       pose (virtue_bound:= konig.finite_product bounded_delta_map bounded_delta_map).
